MirrorCharge!/src/MirrorCharge/Java/Examples/List.v
@@ -1,6 +1,11 @@
+Require Import MirrorCore.syms.SymEnv.
+Require Import MirrorCore.Reify.Reify.
+Require Import MirrorCore.Lambda.Expr.
+Require Import MirrorCore.Lambda.ExprVariables.
+Require Import MirrorCore.RTac.RTac.
+
 Require Import MirrorCharge.Java.JavaType.
 Require Import MirrorCharge.Java.JavaFunc.
-Require Import MirrorCharge.Java.SymEx.
 Require Import MirrorCharge.Java.Reify.
 Require Import MirrorCharge.ModularFunc.OpenFunc.
 Require Import MirrorCharge.ModularFunc.ListFunc.
@@ -11,11 +16,7 @@ Require Import MirrorCharge.AutoSetoidRewrite.
 Require Import MirrorCharge.SetoidRewrite.Base.
 Require Import MirrorCharge.SetoidRewrite.ILSetoidRewrite.
 Require Import MirrorCharge.SetoidRewrite.BILSetoidRewrite.
-
-Require Import MirrorCore.syms.SymEnv.
-Require Import MirrorCore.Reify.Reify.
-Require Import MirrorCore.Lambda.Expr.
-Require Import MirrorCore.RTac.RTac.
+Require Import MirrorCharge.RTac.Apply.
 
 Require Import Java.Examples.ListModel.
 Require Import Java.Examples.ListClass.
@@ -26,6 +27,8 @@ Require Import ExtLib.Core.RelDec.
 
 Require Import MirrorCharge.ModularFunc.ILogicFunc.
 Require Import MirrorCharge.PullConjunct.ILPullConjunct.
+
+Require Import MirrorCharge.Java.SymEx.
 
 Set Printing Width 180.
 
@@ -65,7 +68,7 @@ Definition rw_true (e : expr typ JavaFunc.func)
 (* List rewrite rule type checks *)
 
 Eval vm_compute in typeof_expr nil nil (mkExists tyVal tySasn 
-	(mkStar tySasn (mkPointsto "x" "head" (mkConst tyVal (Var 0))) 
+	(mkStar tySasn (mkPointstoVar "x" "head" (mkConst tyVal (Var 0))) 
 		(mkNode (mkConst tyVal (Var 0)) (mkConst (tyList tyVal) (mkNil tyVal))))).
 
 (* Unfold predicate for list *)
@@ -75,6 +78,8 @@ Definition test_op : expr typ JavaFunc.func :=
   (Inj (inl (inl (inl (inr (of_var "p")))))))).
 
 Eval vm_compute in typeof_expr nil nil test_op.
+
+Eval vm_compute in mkNode (Var 0) (apCons tyVal "n" (Var 0)).
 
 Definition rw_unfold_list (e : expr typ JavaFunc.func) 
 	(rvars : list (RG (expr typ JavaFunc.func))) (rg : RG (expr typ JavaFunc.func)) :
@@ -90,11 +95,31 @@ Definition rw_unfold_list (e : expr typ JavaFunc.func)
         xs =>
           rg_plus
             (rg_bind (unifyRG (@rel_dec (expr typ JavaFunc.func) _ _) rg (RGinj (fEntails tySasn)))
-              (fun _ => rg_ret (mkExists tyVal tySasn (mkStar tySasn (mkPointsto p "head" (mkConst tyVal (Var 0))) (mkNode (mkConst tyVal (Var 0)) (lift 0 1 xs))))
+              (fun _ => rg_ret (mkExists tyVal tySasn (mkStar tySasn (mkPointstoVar p "head" (mkConst tyVal (Var 0))) (mkNode (mkConst tyVal (Var 0)) (lift 0 1 xs))))
               	))
             (rg_bind (unifyRG (@rel_dec (expr typ JavaFunc.func) _ _) rg (RGflip (RGinj (fEntails tySasn))))
-              (fun _ => rg_ret (mkExists tyVal tySasn (mkStar tySasn (mkPointsto p "head" (mkConst tyVal (Var 0))) (mkNode (mkConst tyVal (Var 0)) (lift 0 1 xs))))
+              (fun _ => rg_ret (mkExists tyVal tySasn (mkStar tySasn (mkPointstoVar p "head" (mkConst tyVal (Var 0))) (mkNode (mkConst tyVal (Var 0)) (lift 0 1 xs))))
               ))
+    | App
+         (App (Inj (inl (inl (inl (inr (of_ap (tyList tyVal) tyAsn))))))
+            (App
+               (App (Inj (inl (inl (inl (inr (of_ap tyVal (tyArr (tyList tyVal) tyAsn)))))))
+                  (App (Inj (inl (inl (inl (inr (of_const (tyArr tyVal (tyArr (tyList tyVal) tyAsn)))))))) (Inj (inl (inl (inl (inl (inl (inl (inl (inl 2%positive)))))))))))
+               p))
+         (App
+            (App (Inj (inl (inl (inl (inr (of_ap (tyList tyVal) (tyList tyVal)))))))
+               (App
+                  (App (Inj (inl (inl (inl (inr (of_ap tyVal (tyArr (tyList tyVal) (tyList tyVal))))))))
+                     (App (Inj (inl (inl (inl (inr (of_const (tyArr tyVal (tyArr (tyList tyVal) (tyList tyVal))))))))) (Inj (inl (inl (inl (inl (inr (pCons tyVal)))))))))
+                 x))
+            xs)
+        => rg_plus
+            (rg_bind (unifyRG (@rel_dec (expr typ JavaFunc.func) _ _) rg (RGinj (fEntails tySasn)))
+              (fun _ => rg_ret (mkExists tyVal tySasn (mkStar tySasn (mkPointsto (lift 0 1 p) "val" (lift 0 1 x)) 
+              	(mkStar tySasn (mkPointsto (lift 0 1 p) "next" (mkConst tyVal (Var 0))) (mkNode (mkConst tyVal (Var 0)) (lift 0 1 xs)))))))
+            (rg_bind (unifyRG (@rel_dec (expr typ JavaFunc.func) _ _) rg (RGflip (RGinj (fEntails tySasn))))
+              (fun _ => rg_ret (mkExists tyVal tySasn (mkStar tySasn (mkPointsto (lift 0 1 p) "val" (lift 0 1 x)) 
+              	(mkStar tySasn (mkPointsto (lift 0 1 p) "next" (mkConst tyVal (Var 0))) (mkNode (mkConst tyVal (Var 0)) (lift 0 1 xs)))))))
     | _ => rg_fail
   end.
 
@@ -113,10 +138,65 @@ Eval vm_compute in
     | _ => false
     end.
 
+Require Import MirrorCharge.SetoidRewrite.Base.
+Require Import MirrorCharge.SetoidRewrite.ILSetoidRewrite.
+Require Import MirrorCharge.SetoidRewrite.BILSetoidRewrite.
+Require Import MirrorCharge.SetoidRewrite.EmbedSetoidRewrite.
+
+Require Import MirrorCharge.PullQuant.BILPullQuant.
+Require Import MirrorCharge.PullQuant.ILPullQuant.
+Require Import MirrorCharge.PullQuant.EmbedPullQuant.
+
+Definition pull_quant vars :=
+  setoid_rewrite vars _ (fEntails : typ -> expr typ func) rw_fail
+    (sr_combine il_respects
+               (sr_combine (@il_respects_reflexive typ func _ _ _ ilops _ _)
+                                        (sr_combine bil_respects (sr_combine embed_respects
+                                                    (sr_combine eq_respects refl)))))
+    (sr_combineK  (il_match_plus (fun _ => true) fEq)
+                  (sr_combineK (bil_match_plus fEq) (eil_match_plus fEq))).
+
+Definition PULL_EXISTSR : rtac typ (expr typ func) :=
+  fun tus tvs lus lvs c s e =>
+  match e with
+    | App (App f p) q =>
+      match ilogicS f with
+        | Some (ilf_entails t) => 
+          match pull_quant (getVars c) t q with
+            | Some (q', _) => More s (GGoal (App (App f p) q'))
+            | _ => More s (GGoal e)
+          end
+        | _ => More s (GGoal e)
+      end
+    | _ => More s (GGoal e)
+  end.
+
+Require Import MirrorCharge.ModularFunc.EmbedFunc.
+Require Import MirrorCharge.RTac.Intro.
+
+Definition exists_body : expr typ func :=
+  mkForall tyVal tyProp 
+    (mkForall tyVal tyProp
+    (mkEntails tyProp (mkTrue tyProp) 
+    	(mkAnd tyProp (mkTrue tyProp) (mkExists tyVal tyProp (mkEq tyVal (Var 0) (Var 1)))))).
+
+Eval vm_compute in (THEN (INTRO typ func) PULL_EXISTSR)
+	 nil nil 0 0 (CTop nil nil) (ctx_empty (expr := expr typ JavaFunc.func)) exists_body.
+Eval vm_compute in exists_body.
+
+Require Import MirrorCore.Lambda.Red.
+
+Definition blarf : expr typ func :=
+App (Abs tyVal (App (App (Inj (inl (inl (inl (inl (inl (inr (pEq tyVal)))))))) 
+	(ExprCore.Var 0)) (ExprCore.Var 8))) (Var 3).
+Check beta.
+Eval vm_compute in beta blarf.
+Eval vm_compute in typeof_expr nil nil exists_body.
+
 (* Rewriting with rw_true works *)
 
 Eval vm_compute in 
-  setoid_rewrite _ (fEntails : typ -> expr typ (JavaFunc.func)) rw_true
+  setoid_rewrite nil _ (fEntails : typ -> expr typ (JavaFunc.func)) rw_true
     (sr_combine il_respects
                (sr_combine (@il_respects_reflexive typ (JavaFunc.func) _ _ _ ilops _ _)
                                         (sr_combine bil_respects
@@ -127,7 +207,7 @@ Eval vm_compute in
 (* rewriting with rw_unfold_list does not *)
 
 Eval vm_compute in
-  setoid_rewrite _ (fEntails : typ -> expr typ (JavaFunc.func)) rw_unfold_list
+  setoid_rewrite nil _ (fEntails : typ -> expr typ (JavaFunc.func)) rw_unfold_list
     (sr_combine (il_respects (typ := typ) (func := JavaFunc.func))
                (sr_combine (@il_respects_reflexive typ (JavaFunc.func) _ _ _ ilops _ _)
                                         (sr_combine bil_respects
@@ -136,37 +216,50 @@ Eval vm_compute in
     (fun _ => rw_fail) tySasn (mkList "x" (mkConst (tyList tyVal) (mkNil tyVal))).
 
 Definition add_body := 
-  cseq (calloc "tn" "NodeC") cskip.
-    (*   (cseq (cwrite "tn" "val" (E_var "n"))
+      cseq (calloc "tn" "NodeC")
+         (cseq (cwrite "tn" "val" (E_var "n"))
               (cseq (cread "lst" "this" "head")   
                     (cseq (cwrite "tn" "next" (E_var "lst"))
-                          (cseq (cwrite "this" "head" (E_var "tn")) cskip)))).*)
-(*
+                          (cseq (cwrite "this" "head" (E_var "tn")) cskip)))).
+
 Definition testAdd :=
 		(mkForall (tyList tyVal) tyProp
 		  	(mkEntails tySpec (mkProgEq (mkProg ListProg))
 		  	           (mkTriple (mkList "this" (mkConst (tyList tyVal) (Var 0)))
 		  	           			 (mkCmd add_body)
 		  	           			 (mkList "this" (apCons tyVal "n" (mkConst (tyList tyVal) (Var 0))))))).
-*)
-Definition testAdd :=
-		(mkForall (tyList tyVal) tyProp
-		  	(mkEntails tySpec (mkProgEq (mkProg ListProg))
-		  	           (mkTriple (mkList "this" (mkConst (tyList tyVal) (Var 0)))
-		  	           			 (mkCmd add_body)
-		  	           			 (mkFalse tySasn)))).
+
 
 Set Printing Depth 100.  	           		
 
+Fixpoint goal_to_expr (g : Goal typ (expr typ func)) : list (expr typ func) :=
+  match g with
+    | GGoal e => e::nil
+    | GSolved => nil
+    | GExs _ _ g => goal_to_expr g
+    | GHyp _ g => goal_to_expr g
+    | GAll _ g => goal_to_expr g
+    | GConj_ l r => (goal_to_expr l) ++ (goal_to_expr r)
+  end.
+
 Require Import MirrorCharge.RTac.Intro.
 Require Import MirrorCharge.RTac.Instantiate.
-	 
-Definition runTac (tac : expr typ JavaFunc.func) rw := 
-   THEN (THEN (REPEAT 1000 (INTRO typ JavaFunc.func subst)) (runOnGoals (symE rw))) 
-	(runOnGoals (INSTANTIATE typ JavaFunc.func subst))
-	 nil nil 0 0 (@SubstI.empty (ctx_subst subst CTop) (expr typ JavaFunc.func) _) tac.
+Require Import MirrorCharge.RTac.Cancellation.
+Print ent_exists_right_lemma.
+Print pull_exists_lemma.
+Definition runTac2 (tac : expr typ JavaFunc.func) rw := 
+     (THEN (THEN (THEN (THEN (THEN (THEN (THEN (REPEAT 1000 (INTRO typ JavaFunc.func)) (symE rw)) 
+	(INSTANTIATE typ JavaFunc.func)) 
+		(TRY (THEN (THEN (THEN (APPLY typ JavaFunc.func ent_exists_right_lemma) (INSTANTIATE typ JavaFunc.func))
+			(INTRO typ JavaFunc.func)) BETA)))
+	 (STEP_REWRITE rw))  PULL_EXISTSR)
+		((THEN (THEN (THEN (APPLY typ JavaFunc.func ent_exists_right_lemma) (INSTANTIATE typ JavaFunc.func))
+			(INTRO typ JavaFunc.func)) BETA)))
+			
+     (CANCELLATION typ func tySasn is_pure))
+	 nil nil 0 0 (CTop nil nil) (ctx_empty (expr := expr typ JavaFunc.func)) tac.
 
-Eval vm_compute in runTac testAdd rw_unfold_list.
+Time Eval vm_compute in runTac2 testAdd rw_unfold_list.
 
 Time Eval vm_compute in 
 	match (runTac testAdd rw_unfold_list) with
@@ -178,115 +271,3 @@ Time Eval vm_compute in
 		       )
 		| _ => None
 	end.
-
-Definition g : Goal typ (expr typ JavaFunc.func) :=
-GAll (tyList tyVal)
-                  (GAll tyVal
-                     (GGoal
-                        (App
-                           (App (Inj (inl (inl (inl (inl (inl (inl (inl (inr (ilf_entails tySpec))))))))))
-                              (App (Inj (inr pProgEq))
-                                 (Inj
-                                    (inr
-                                       (pProg
-                                          {|
-                                          Program.p_classes := ("List",
-                                                               {|
-                                                               Program.c_fields := "head" :: nil;
-                                                               Program.c_methods := ("add",
-                                                                    {|
-                                                                    Program.m_params := "this" :: "n" :: nil;
-                                                                    Program.m_body := "tn" N=  alloc "NodeC";;
-                                                                    "tn" ["val"]W=E_var "n";; "lst" R= "this" ["head"];; "tn" ["next"]W=E_var "lst";; "this" ["head"]W=E_var "tn";
-                                                                    Program.m_ret := E_val 0%Z |}) :: nil |})
-                                                               :: ("NodeC", {| Program.c_fields := "val" :: "next" :: nil; Program.c_methods := nil |}) :: nil |})))))
-                           (App
-                              (App
-                                 (App (Inj (inr pTriple))
-                                    (App
-                                       (App (Inj (inl (inl (inl (inl (inl (inl (inl (inr (ilf_and tySasn))))))))))
-                                          (App (Inj (inl (inl (inr (EmbedFunc.eilf_embed tyPure tySasn)))))
-                                             (App
-                                                (App (Inj (inl (inl (inl (inl (inl (inl (inl (inr (ilf_and tyPure))))))))))
-                                                   (App
-                                                      (App (Inj (inl (inl (inl (inr (of_ap tyVal tyProp))))))
-                                                         (App
-                                                            (App (Inj (inl (inl (inl (inr (of_ap tyClass (tyArr tyVal tyProp)))))))
-                                                               (App (Inj (inl (inl (inl (inr (of_const (tyArr tyClass (tyArr tyVal tyProp)))))))) (Inj (inr pTypeOf))))
-                                                            (App (Inj (inl (inl (inl (inr (of_const tyClass)))))) (Inj (inr (pClass "NodeC"))))))
-                                                      (App (Inj (inl (inl (inl (inr of_stack_get))))) (Inj (inl (inl (inl (inr (of_var "tn")))))))))
-                                                (App
-                                                   (App (Inj (inl (inl (inl (inr (of_ap tyVal tyProp))))))
-                                                      (App
-                                                         (App (Inj (inl (inl (inl (inr (of_ap tyVal (tyArr tyVal tyProp)))))))
-                                                            (App (Inj (inl (inl (inl (inr (of_const (tyArr tyVal (tyArr tyVal tyProp))))))))
-                                                               (Inj (inl (inl (inl (inl (inl (inr (pEq tyVal))))))))))
-                                                         (App (Inj (inl (inl (inl (inr of_stack_get))))) (Inj (inl (inl (inl (inr (of_var "tn")))))))))
-                                                   (App (Inj (inl (inl (inl (inr (of_const tyVal)))))) (Var 1))))))
-                                       (App
-                                          (App (Inj (inl (inl (inl (inl (inl (inl (inr (bilf_star tySasn)))))))))
-                                             (App
-                                                (App (Inj (inl (inl (inl (inr (of_ap tyVal tyAsn))))))
-                                                   (App
-                                                      (App (Inj (inl (inl (inl (inr (of_ap tyField (tyArr tyVal tyAsn)))))))
-                                                         (App
-                                                            (App (Inj (inl (inl (inl (inr (of_ap tyVal (tyArr tyField (tyArr tyVal tyAsn))))))))
-                                                               (App (Inj (inl (inl (inl (inr (of_const (tyArr tyVal (tyArr tyField (tyArr tyVal tyAsn)))))))))
-                                                                  (Inj (inr pPointsto))))
-                                                            (App (Inj (inl (inl (inl (inr of_stack_get))))) (Inj (inl (inl (inl (inr (of_var "tn")))))))))
-                                                      (App (Inj (inl (inl (inl (inr (of_const tyField)))))) (Inj (inr (pField "val"))))))
-                                                (App (Inj (inl (inl (inl (inr (of_const tyVal)))))) (Inj (inr (pVal null))))))
-                                          (App
-                                             (App (Inj (inl (inl (inl (inl (inl (inl (inr (bilf_star tySasn)))))))))
-                                                (App
-                                                   (App (Inj (inl (inl (inl (inr (of_ap tyVal tyAsn))))))
-                                                      (App
-                                                         (App (Inj (inl (inl (inl (inr (of_ap tyField (tyArr tyVal tyAsn)))))))
-                                                            (App
-                                                               (App (Inj (inl (inl (inl (inr (of_ap tyVal (tyArr tyField (tyArr tyVal tyAsn))))))))
-                                                                  (App 
-                                                                    (Inj (inl (inl (inl (inr (of_const (tyArr tyVal (tyArr tyField (tyArr tyVal tyAsn)))))))))
-                                                                    (Inj (inr pPointsto))))
-                                                               (App (Inj (inl (inl (inl (inr of_stack_get))))) (Inj (inl (inl (inl (inr (of_var "tn")))))))))
-                                                         (App (Inj (inl (inl (inl (inr (of_const tyField)))))) (Inj (inr (pField "next"))))))
-                                                   (App (Inj (inl (inl (inl (inr (of_const tyVal)))))) (Inj (inr (pVal null))))))
-                                             (App
-                                                (App (Inj (inl (inl (inl (inr (of_apply_subst tyAsn))))))
-                                                   (App
-                                                      (App (Inj (inl (inl (inl (inl (inl (inl (inr (bilf_star tySasn)))))))))
-                                                         (App
-                                                            (App (Inj (inl (inl (inl (inr (of_ap tyVal tyAsn))))))
-                                                               (App
-                                                                  (App 
-                                                                    (Inj (inl (inl (inl (inr (of_ap tyField (tyArr tyVal tyAsn)))))))
-                                                                    (App
-                                                                    (App 
-                                                                    (Inj (inl (inl (inl (inr (of_ap tyVal (tyArr tyField (tyArr tyVal tyAsn))))))))
-                                                                    (App 
-                                                                    (Inj (inl (inl (inl (inr (of_const (tyArr tyVal (tyArr tyField (tyArr tyVal tyAsn)))))))))
-                                                                    (Inj (inr pPointsto))))
-                                                                    (App (Inj (inl (inl (inl (inr of_stack_get))))) (Inj (inl (inl (inl (inr (of_var "this")))))))))
-                                                                  (App (Inj (inl (inl (inl (inr (of_const tyField)))))) (Inj (inr (pField "head"))))))
-                                                            (App (Inj (inl (inl (inl (inr (of_const tyVal)))))) (Var 1))))
-                                                      (App
-                                                         (App (Inj (inl (inl (inl (inr (of_ap (tyList tyVal) tyAsn))))))
-                                                            (App
-                                                               (App (Inj (inl (inl (inl (inr (of_ap tyVal (tyArr (tyList tyVal) tyAsn)))))))
-                                                                  (App 
-                                                                    (Inj (inl (inl (inl (inr (of_const (tyArr tyVal (tyArr (tyList tyVal) tyAsn))))))))
-                                                                    (Inj (inl (inl (inl (inl (inl (inl (inl (inl 2%positive)))))))))))
-                                                               (App (Inj (inl (inl (inl (inr (of_const tyVal)))))) (Var 1))))
-                                                         (App (Inj (inl (inl (inl (inr (of_const (tyList tyVal))))))) (Var 0)))))
-                                                (App (App (Inj (inl (inl (inl (inr of_single_subst))))) (App (Inj (inl (inl (inl (inr (of_const tyVal)))))) (Var 1)))
-                                                   (Inj (inl (inl (inl (inr (of_var "tn")))))))))))) 
-                                 (Inj (inl (inl (inl (inl (inl (inl (inl (inr (ilf_false tySasn))))))))))) 
-                              (Inj (inr (pCmd Skip))))))).
-
-Time Eval vm_compute in 
-match goalD nil nil g with
-		          | Some _ => None
-		          | _ => Some g
-		      
-	end.
-
-
