MirrorCharge!/src/MirrorCharge/RTac/Apply.v
@@ -9,20 +9,20 @@ Require Import MirrorCore.SubstI.
 Require Import MirrorCore.Lambda.ExprUnify_simul.
 
 Section AutoTac.
-	Context {typ func subst : Type}.
+	Context {typ func : Type}.
 	Context {RType_typ : RType typ}.
-	Context {Typ2_typ : Typ2 RType_typ Fun}.
 	Context {Typ0_typ : Typ0 RType_typ Prop}.
+	Context {Typ2_typ : Typ2 RType_typ Fun}.
 	Context {RSym_func : @RSym _ RType_typ func}.
-	Context {SS : SubstI.Subst subst (expr typ func)}.
-	Context {SU : SubstI.SubstUpdate subst (expr typ func)}.
+	Context {EU : ExprUVar (expr typ func)}.
+	Context {MA : MentionsAny (expr typ func)}.
 
-Definition APPLY := @APPLY typ (expr typ func) subst _ _ _ _ UVar
+Definition APPLY := @APPLY typ (expr typ func) RType_typ Typ0_typ EU MA
                     (@vars_to_uvars _ _)
-                    (fun _ _ _ tus tvs n l r t s =>
-                       @exprUnify _ _ _ _ _ _ _ _ 10 tus tvs n s l r t)
-                    (@instantiate _ _).
+                    (fun subst SS SU tus tvs n l r t s =>
+                       @exprUnify subst typ func RType_typ RSym_func Typ2_typ 
+                                  SS SU 10 tus tvs n s l r t).
 
 End AutoTac.
-Check APPLY.
-Implicit Arguments APPLY [[RType_typ] [Typ2_typ] [Typ0_typ] [RSym_func] [SS] [SU]].
+
+Implicit Arguments APPLY [[RType_typ] [Typ2_typ] [Typ0_typ] [RSym_func] [EU] [MA]].
